coq-osiris/theories/program_logic/pure/pure_rules.v
@@ -56,6 +56,7 @@ Section pure_rules.
     intros; eapply pure_ret; eauto.
   Qed.
 
+
   Lemma pure_returns (a : val) (k : val -> micro val E) φ ψ:
     pure (k a) φ ψ ->
     returns (λ v : val, pure (k v) φ ψ) a.
@@ -319,6 +320,14 @@ Section pure_rules.
 End pure_rules.
 
 Section pure_rules_variant.
+
+  (* When a [val] is returned, there is no need for [encode]. *)
+  Lemma pure_ret_val `{Encode A} {E} (a : val) (ϕ : A -> Prop) ψ :
+    returns ϕ a ->
+    pure (E := E) (ret a) ϕ ψ.
+  Proof.
+    intros. returns_eauto. by eapply pure_ret.
+  Qed.
 
   Lemma pure_ret_eq_val {E} {A} `{EncA: Encode A} (a : A) ψ :
     pure (E := E) (ret #a) (λ a', a' = a) ψ.
